In forward.v, clean up the semax_load_tac.  Previously there were three cases:   (Sset _ (Efield (Ederef _ _) _ _))   (Sset _ (Efield _ _ _))   (Sset _ (Ederef _ _))
Now the first case has been eliminated, subsumed into the second case.
This will help when we want to add more support for array subscripting.

What made this slightly difficult is that we need extra work
to eliminate instances of "force_ptr", i.e. that the expression being
dereferenced really is a pointer.  

Next, the store_field_tac really ought to be cleaned up in just the same way.

floyd/loadstore_lemmas.v
@@ -467,7 +467,27 @@ apply sepcon_derives; auto.
 go_lowerx. apply field_mapsto_field_mapsto_.
 Qed.
 
-Lemma semax_load_field'':
+Definition force_eq ( x y: val) := force_ptr x = force_ptr y.
+
+
+Lemma force_force_eq:
+  forall v, force_ptr (force_ptr v) = force_ptr v.
+Proof. intros. destruct v; reflexivity. Qed.
+
+Lemma force_eq1: forall v w, force_eq v w -> force_eq (force_ptr v) w .
+Proof. unfold force_eq; intros; rewrite force_force_eq; auto. Qed.
+
+Lemma force_eq2: forall v w, force_eq v w -> force_eq v (force_ptr w).
+Proof. unfold force_eq; intros; rewrite force_force_eq; auto. Qed.
+
+Lemma force_eq0: forall v w, v=w -> force_eq v w.
+Proof. intros. subst. reflexivity. Qed.
+
+Ltac force_eq_tac := repeat first [simple apply force_eq1 | simple apply force_eq2];
+                                 try apply force_eq0;
+                                 first [assumption |  reflexivity].
+
+Lemma semax_load_field''force:
 forall Espec (Delta: tycontext) n sh id t1 fld P Q R e1 v1 v2 t2 i2 sid fields ,
     t1 = Tstruct sid fields noattr ->
     typeof e1 = t1 ->
@@ -475,8 +495,9 @@ forall Espec (Delta: tycontext) n sh id t1 fld P Q R e1 v1 v2 t2 i2 sid fields ,
    t2 = type_of_field
              (unroll_composite_fields sid (Tstruct sid fields noattr) fields) fld ->
      Cop.classify_cast t2 t2 = Cop.cast_case_neutral ->
-     PROPx P (LOCALx (tc_environ Delta :: Q) (SEPx R)) |-- local (tc_lvalue Delta e1) ->
-    PROPx P (LOCALx (tc_environ Delta :: Q) (SEPx R)) |-- local (`eq v1 (eval_lvalue e1)) ->
+     PROPx P (LOCALx (tc_environ Delta :: `isptr (eval_lvalue e1) :: Q) (SEPx R)) 
+                           |-- local (tc_lvalue Delta e1) ->
+    PROPx P (LOCALx (tc_environ Delta :: Q) (SEPx R)) |-- local (`force_eq v1 (eval_lvalue e1)) ->
     nth_error R n = Some (`(field_mapsto sh t1 fld) v1 v2) ->
     @semax Espec Delta 
        (|> PROPx P (LOCALx Q (SEPx R)))
@@ -487,7 +508,6 @@ forall Espec (Delta: tycontext) n sh id t1 fld P Q R e1 v1 v2 t2 i2 sid fields ,
                 (SEPx 
                   (map (subst id (`old))
                     (replace_nth n R (`(field_mapsto sh t1 fld) (eval_lvalue e1) v2))))))).
-Proof.
 intros. rename H3 into CC.
 eapply semax_pre_post;
   [ | |  apply (semax_load_field Espec Delta sh id t1 fld (PROPx P (LOCALx Q (SEPx (replace_nth n R emp)))) e1
@@ -498,10 +518,7 @@ end.
 rewrite later_andp; apply andp_derives; auto; apply now_later.
 apply later_derives.
 rewrite insert_local.
-rewrite (local_andp_lemma _ _ H4).
-rewrite (local_andp_lemma _ _ H5).
-rewrite <- insert_local.
-assert (PROPx P (LOCALx Q (SEPx R)) |-- local (`isptr v1)).
+assert (H3: PROPx P (LOCALx Q (SEPx R)) |-- local (`isptr v1)).
 clear - H6.
 go_lowerx.
 unfold_lift in H6.
@@ -509,9 +526,29 @@ revert R H6; induction n; destruct R; simpl; intros; inv H6.
 rewrite field_mapsto_isptr. clear; normalize.
 apply derives_trans with (TT * (!!isptr (v1 rho) && TT)).
 apply sepcon_derives; auto. rewrite andp_TT; auto. normalize.
+assert (H4':  PROPx P
+       (LOCALx (tc_environ Delta :: Q) (SEPx R)) |-- local (tc_lvalue Delta e1)).
+eapply derives_trans; [ | apply H4].
+clear - H3 H5.
+rewrite (local_andp_lemma _ _ H5).
+repeat rewrite <- insert_local.
+forget (PROPx P (LOCALx Q (SEPx R))) as PQR.
+go_lowerx. apply andp_right; auto. 
+eapply derives_trans; [ apply H3 |].
+unfold local, lift1. apply prop_derives.
+unfold_lift;intros. unfold force_eq in H.
+rewrite (isptr_force_ptr _ H1) in H. rewrite H in H1.
+destruct (eval_lvalue e1 rho); inv H1; simpl; auto.
+clear H4.
+rewrite (local_andp_lemma _ _ H4').
+rewrite (local_andp_lemma _ _ H5).
+rewrite <- insert_local.
  rewrite (local_andp_lemma _ _ H3).
 go_lowerx.
-rewrite <- H8.
+unfold force_eq in H8.
+rewrite <- field_mapsto_force_ptr.
+rewrite <- H7.
+rewrite isptr_force_ptr by auto.
 clear - H6. rename H6 into H5.
 clear - H5; revert R H5; induction n; destruct R; simpl; intros; inv H5.
 rewrite emp_sepcon; apply sepcon_derives; auto.
@@ -535,6 +572,36 @@ rewrite sepcon_assoc.
 apply sepcon_derives; auto.
 Qed.
 
+
+Lemma semax_load_field'':
+forall Espec (Delta: tycontext) n sh id t1 fld P Q R e1 v1 v2 t2 i2 sid fields ,
+    t1 = Tstruct sid fields noattr ->
+    typeof e1 = t1 ->
+        (temp_types Delta) ! id = Some (t2,i2) ->
+   t2 = type_of_field
+             (unroll_composite_fields sid (Tstruct sid fields noattr) fields) fld ->
+     Cop.classify_cast t2 t2 = Cop.cast_case_neutral ->
+     PROPx P (LOCALx (tc_environ Delta :: Q) (SEPx R)) |-- local (tc_lvalue Delta e1) ->
+    PROPx P (LOCALx (tc_environ Delta :: Q) (SEPx R)) |-- local (`eq v1 (eval_lvalue e1)) ->
+    nth_error R n = Some (`(field_mapsto sh t1 fld) v1 v2) ->
+    @semax Espec Delta 
+       (|> PROPx P (LOCALx Q (SEPx R)))
+       (Sset id (Efield e1 fld t2))
+       (normal_ret_assert 
+        (EX old:val,
+          PROPx P (LOCALx (`eq (eval_id id) (subst id (`old) v2) :: map (subst id (`old)) Q)
+                (SEPx 
+                  (map (subst id (`old))
+                    (replace_nth n R (`(field_mapsto sh t1 fld) (eval_lvalue e1) v2))))))).
+Proof.
+intros; eapply semax_load_field''force; eauto.
+do 2 rewrite <- insert_local. rewrite <- andp_assoc.
+rewrite (andp_comm (local _)). rewrite andp_assoc. rewrite insert_local.
+apply andp_left2.
+auto.
+admit.  (* straightforward *)
+Qed.
+
 Lemma semax_load_field_deref'':
 forall Espec (Delta: tycontext) n sh id t1 fld P Q R e1 v1 v2 t2 i2 sid fields ,
     t1 = Tstruct sid fields noattr ->
@@ -556,7 +623,7 @@ forall Espec (Delta: tycontext) n sh id t1 fld P Q R e1 v1 v2 t2 i2 sid fields ,
                   (map (subst id (`old))
                     (replace_nth n R (`(field_mapsto sh t1 fld) (eval_expr e1) v2))))))).
 Proof.
-intros. rename H3 into CC.
+intros; rename H3 into CC.
 eapply semax_pre_post;
   [ | |  apply (semax_load_field Espec Delta sh id t1 fld (PROPx P (LOCALx Q (SEPx (replace_nth n R emp)))) (Ederef e1 t1)
    v2 t2 i2 sid fields)]; auto; try congruence.
